coq/SimpleFormInterpretation.v
@@ -4,6 +4,9 @@ Require Import Koika.Environments Koika.SimpleForm Koika.TypeInference
 Require Import Koika.BitsToLists.
 From RecordUpdate Require Import RecordSet.
 Import RecordSetNotations.
+Require Import Sact.
+Require Import Coq.Sorting.Sorted.
+Require Import Coq.Sorting.Mergesort.
 
 Section SimpleFormInterpretation.
   Context {pos_t reg_t ext_fn_t rule_name_t: Type}.
@@ -15,7 +18,7 @@ Section SimpleFormInterpretation.
   Context (R: reg_t -> type).
   Context (Sigma: ext_fn_t -> ExternalSignature).
 
-  Definition uact := @uaction pos_t string string reg_t ext_fn_t.
+  Definition uact := @daction pos_t string string reg_t ext_fn_t.
   Definition schedule := scheduler pos_t rule_name_t.
   Definition ext_funs_defs :=
     forall f: ext_fn_t, BitsToLists.val -> BitsToLists.val.
@@ -24,143 +27,1292 @@ Section SimpleFormInterpretation.
   Context (r: UREnv).
   Context (sigma: ext_funs_defs).
 
-  Definition const_nil :=
-    @UConst pos_t string string reg_t ext_fn_t (bits_t 0) (Bits.of_nat 0 0).
-  Definition const_false :=
-    @UConst pos_t string string reg_t ext_fn_t (bits_t 1) (Bits.of_nat 1 0).
-  Definition const_true :=
-    @UConst pos_t string string reg_t ext_fn_t (bits_t 1) (Bits.of_nat 1 1).
+  Definition sact := sact (ext_fn_t:=ext_fn_t).
 
-  Fixpoint contains_vars (e: uact) : bool :=
+  Fixpoint contains_vars (e: sact) : bool :=
     match e with
-    | UBinop ufn a1 a2 => orb (contains_vars a1) (contains_vars a2)
-    | UUnop ufn a1 => contains_vars a1
-    | UVar v => true
-    | UIf cond tb fb =>
+    | SConst _ => false
+    | SBinop ufn a1 a2 => orb (contains_vars a1) (contains_vars a2)
+    | SUnop ufn a1 => contains_vars a1
+    | SVar v => true
+    | SIf cond tb fb =>
       orb (contains_vars cond) (orb (contains_vars tb) (contains_vars fb))
-    | _ => false (* URead *)
+    | SExternalCall _ a => contains_vars a
     end.
 
-  Fixpoint replace_all_occurrences_in_uact (ua: uact) (from: string) (to: val)
-  : uact :=
+  Fixpoint replace_all_occurrences_in_sact (ua: sact) (from: nat) (to: val)
+  : sact :=
     match ua with
-    | UBinop ufn a1 a2 =>
-      UBinop
-        ufn (replace_all_occurrences_in_uact a1 from to)
-        (replace_all_occurrences_in_uact a2 from to)
-    | UUnop ufn a1 => UUnop ufn (replace_all_occurrences_in_uact a1 from to)
-    | UVar v =>
-      if (String.eqb v from) then
-        let bl := ubits_of_value to in
-        UConst (tau := bits_t (List.length bl)) (vect_of_list bl)
-      else UVar v
-    | UIf cond tb fb =>
-      UIf
-        (replace_all_occurrences_in_uact cond from to)
-        (replace_all_occurrences_in_uact tb from to)
-        (replace_all_occurrences_in_uact fb from to)
-    | _ => ua
+    | SBinop ufn a1 a2 =>
+      SBinop
+        ufn (replace_all_occurrences_in_sact a1 from to)
+        (replace_all_occurrences_in_sact a2 from to)
+    | SUnop ufn a1 => SUnop ufn (replace_all_occurrences_in_sact a1 from to)
+    | SVar v =>
+      if eq_dec v from then SConst to
+      else SVar v
+    | SIf cond tb fb =>
+      SIf
+        (replace_all_occurrences_in_sact cond from to)
+        (replace_all_occurrences_in_sact tb from to)
+        (replace_all_occurrences_in_sact fb from to)
+    | SConst c => SConst c
+    | SExternalCall ufn a => SExternalCall ufn (replace_all_occurrences_in_sact a from to)
     end.
 
   Definition replace_all_occurrences_in_vars
-    (vars: var_value_map) (from: string) (to: val)
+    (vars: var_value_map) (from: nat) (to: val)
   : var_value_map :=
     map
-      (fun '(reg, ua) => (reg, replace_all_occurrences_in_uact ua from to))
+      (fun '(reg, (t, ua)) => (reg, (t, replace_all_occurrences_in_sact ua from to)))
       vars.
 
-  Definition replace_all_occurrences_in_extcalls
-    (extc: extcall_log) (from: string) (to: val)
-  : extcall_log :=
-    map
-      (fun '(en, ei) => (en, {|
-        econd := replace_all_occurrences_in_uact (econd ei) from to;
-        earg := replace_all_occurrences_in_uact (earg ei) from to;
-        ebind := ebind ei |}))
-      extc.
-
   (* TODO simplify as well: initial simpl pass then whenever change *)
-  Definition replace_all_occurrences (sf: simple_form) (from: string) (to: val)
+  Definition simple_form := simple_form (reg_t:=reg_t) (ext_fn_t:=ext_fn_t).
+  Definition replace_all_occurrences (sf: simple_form) (from: nat) (to: val)
   : simple_form := {|
     final_values := final_values sf;
-    vars := replace_all_occurrences_in_vars (vars sf) from to;
-    external_calls :=
-      replace_all_occurrences_in_extcalls (external_calls sf) from to |}.
+    vars := replace_all_occurrences_in_vars (vars sf) from to; |}.
 
   (* TODO use coq record update here as well *)
   (* TODO variable in environment instead of inlining *)
 
-  Definition remove_by_name_extc
-    (sf: @simple_form pos_t reg_t ext_fn_t) (name: string)
-  : simple_form := {|
-    final_values := final_values sf;
-    vars := vars sf;
-    external_calls :=
-      filter (fun '(_, ei) => eqb (ebind ei) name) (external_calls sf) |}.
-
   Definition remove_by_name_var
-    (sf: @simple_form pos_t reg_t ext_fn_t) (name: string)
-  : simple_form := {|
-    final_values := final_values sf;
-    vars := filter (fun '(n, _) => eqb n name) (vars sf);
-    external_calls := external_calls sf |}.
+             (sf: simple_form) (name: nat) : simple_form :=
+    {|
+      final_values := final_values sf;
+      vars := filter (fun '(n, _) => negb (beq_dec n name)) (vars sf);
+    |}.
 
-  Definition set_cond_true_by_name
-    (sf: @simple_form pos_t reg_t ext_fn_t) (name: string)
-  : simple_form := {|
-    final_values := final_values sf;
-    vars := vars sf;
-    external_calls :=
-      map
-        (fun '(efn, ei) =>
-          if eqb name (ebind ei)
-          then (
-            efn,
-            {| econd := UConst (tau := bits_t 1) (Bits.of_nat 1 1);
-               earg := earg ei; ebind := ebind ei |})
-          else (efn, ei))
-        (external_calls sf) |}.
 
-  Definition inlining_pass (sf: @simple_form pos_t reg_t ext_fn_t)
-  : simple_form * list (string * val) :=
+  Fixpoint eval_sact (vars: var_value_map) (a: sact) (fuel: nat) : option val :=
+    match fuel with
+    | O => None
+    | S fuel =>
+        match a with
+        | SConst v => Some v
+        | SVar v =>
+            let/opt2 t, vv := list_assoc vars v in
+            eval_sact vars vv fuel
+        | SIf c t f =>
+            let/opt v := eval_sact vars c fuel in
+            match v with
+            | Bits 1 [b] =>
+                if b then eval_sact vars t fuel
+                else eval_sact vars f fuel
+            | _ => None
+            end
+        | SUnop ufn a =>
+            let/opt v := eval_sact vars a fuel in
+            sigma1 ufn v
+        | SBinop ufn a1 a2 =>
+            let/opt v1 := eval_sact vars a1 fuel in
+            let/opt v2 := eval_sact vars a2 fuel in
+            sigma2 ufn v1 v2
+        | SExternalCall ufn a =>
+            let/opt v := eval_sact vars a fuel in
+            Some (sigma ufn v)
+        end
+    end.
+
+  Fixpoint max_var (vars: var_value_map (ext_fn_t:=ext_fn_t)) :=
+    match vars with
+      [] => O
+    | (n,_)::vars => max n (max_var vars)
+    end.
+
+  Lemma vvs_range_max_var:
+    forall vars,
+      vvs_range vars (S (max_var vars)).
+  Proof.
+    red; intros.
+    apply Sact.list_assoc_in in H.
+    red.
+    revert x y H.
+    induction vars; simpl; intros; eauto. easy.
+    destruct H. subst. lia.
+    eapply IHvars in H. destr. lia.
+  Qed.
+
+  Open Scope nat.
+
+  Lemma eval_sact_more_fuel:
+    forall n1 vvs a v n2,
+      eval_sact vvs a n1 = Some v ->
+      n1 <= n2 ->
+      eval_sact vvs a n2 = Some v.
+  Proof.
+    induction n1; simpl; intros; eauto. easy.
+    destruct n2; simpl. lia.
+    unfold opt_bind in *.
+    assert (n1 <= n2) by lia.
+    repeat destr_in H; inv H; eauto.
+    - erewrite IHn1; eauto.
+    - erewrite IHn1; eauto.
+      erewrite IHn1; eauto.
+    - erewrite IHn1; eauto.
+      simpl. erewrite IHn1; eauto.
+    - erewrite IHn1; eauto.
+    - erewrite IHn1; eauto.
+      erewrite IHn1; eauto.
+    - erewrite IHn1; eauto.
+  Qed.
+
+  Fixpoint vvs_size (vvs:var_value_map) m : nat :=
+    match vvs with
+      [] => O
+    | (n,(t,a))::vvs =>
+        if lt_dec n m then
+          size_sact (ext_fn_t:=ext_fn_t) a + vvs_size vvs m
+        else vvs_size vvs m
+    end.
+
+  Lemma vvs_size_le1:
+    forall vvs var n,
+      var < n ->
+      vvs_size vvs var  <= vvs_size vvs n.
+  Proof.
+    induction vvs; simpl; intros. easy.
+    repeat destr; try lia.
+    - clear Heqs0. apply IHvvs in H. lia.
+    - apply IHvvs in H. lia.
+    - apply IHvvs in H. lia.
+  Qed.
+
+  Lemma vvs_size_le2:
+    forall vvs a var t n,
+      var < n ->
+      list_assoc vvs var = Some (t, a) ->
+      vvs_size vvs var + size_sact a <= vvs_size vvs n.
+  Proof.
+    induction vvs; simpl; intros. easy.
+    repeat destr_in H0. inv H0.
+    - destr. lia. destr.
+      cut (vvs_size vvs n0 <= vvs_size vvs n).
+      2: eapply vvs_size_le1; eauto. lia.
+    - destr.
+      generalize (IHvvs _ _ _ _ H H0).
+      generalize (vvs_size_le1 vvs _ _ H). intros.
+      repeat destr; try lia.
+  Qed.
+
+  Lemma interp_sact_eval_sact_aux:
+    forall (vvs: var_value_map) (VSV: vvs_smaller_variables vvs),
+    forall a v,
+      interp_sact (sigma:=sigma) vvs a v ->
+      forall n, (forall var, var_in_sact a var -> var < n) ->
+      exists m, eval_sact vvs a (m + size_sact a) = Some v /\ m <= n + vvs_size vvs n.
+  Proof.
+    induction 2; simpl; intros; eauto.
+    - destruct (IHinterp_sact var) as (m1 & I1 & LE1). intros; eapply VSV. eauto. auto.
+      eexists. split. rewrite Nat.add_1_r. simpl. rewrite H; simpl; eauto.
+      assert (var < n). eapply H1. constructor.
+      generalize (vvs_size_le2 vvs _ _ _ n H2 H). lia.
+    - exists 0; split; simpl; eauto.  lia. 
+    - edestruct IHinterp_sact1 as (m1 & I1 & LE1).
+      intros; eapply H1. apply var_in_if_cond; eauto.
+      edestruct IHinterp_sact2 as (m2 & I2 & LE2).
+      intros; eapply H1. destruct b. apply var_in_if_true; eauto. apply var_in_if_false; eauto.
+      exists ((max m1 m2)). split.
+      rewrite Nat.add_succ_r.
+      simpl.
+      erewrite eval_sact_more_fuel; eauto. 2: lia. simpl.
+      destruct b; eapply eval_sact_more_fuel; eauto. lia. lia. lia.
+    - edestruct IHinterp_sact as (m1 & I1 & LE1).
+      intros; eapply H1. econstructor; eauto.
+      exists m1; rewrite Nat.add_succ_r. simpl. rewrite I1.
+      split; simpl; eauto.
+    - edestruct IHinterp_sact1 as (m1 & I1 & LE1).
+      intros; eapply H2. econstructor; eauto.
+      edestruct IHinterp_sact2 as (m2 & I2 & LE2).
+      intros; eapply H2. eapply var_in_sact_binop_2; eauto.
+      exists (max m1 m2); rewrite Nat.add_succ_r. simpl.
+      erewrite eval_sact_more_fuel; eauto. 2: lia. simpl.
+      erewrite eval_sact_more_fuel; eauto. 2: lia. simpl.
+      split; simpl; eauto. lia.
+    - edestruct IHinterp_sact as (m1 & I1 & LE1).
+      intros; eapply H0. econstructor; eauto.
+      exists m1; rewrite Nat.add_succ_r. simpl. rewrite I1.
+      split; simpl; eauto.
+  Qed.
+
+  Lemma interp_sact_eval_sact:
+    forall (vvs: var_value_map) (VSV: vvs_smaller_variables vvs),
+    forall a v t,
+      wt_sact (Sigma:=Sigma) vvs a t ->
+      interp_sact (sigma:=sigma) vvs a v ->
+      eval_sact vvs a (S (max_var vvs) + vvs_size vvs (S (max_var vvs)) + size_sact a) = Some v.
+  Proof.
+    intros.
+    generalize (vvs_range_max_var vvs). intro VR.
+    generalize (wt_sact_valid_vars vvs _ VR _ _ H). intro VALID.
+    generalize (interp_sact_eval_sact_aux _ VSV a v H0 _ VALID).
+    intros (m & EVAL & LE).
+    eapply eval_sact_more_fuel. eauto. lia.
+  Qed.
+
+  Definition do_eval_sact vvs a :=
+    eval_sact vvs a (S (max_var vvs) + vvs_size vvs (S (max_var vvs)) + size_sact a).
+
+  Lemma interp_sact_do_eval_sact:
+    forall (vvs: var_value_map) (VSV: vvs_smaller_variables vvs),
+    forall a v t,
+      wt_sact (Sigma:=Sigma) vvs a t ->
+      interp_sact (sigma:=sigma) vvs a v ->
+      do_eval_sact vvs a = Some v.
+  Proof.
+    intros.
+    eapply interp_sact_eval_sact; eauto.
+  Qed.
+
+  Lemma eval_sact_interp_sact:
+    forall vvs fuel a v,
+      eval_sact vvs a fuel = Some v ->
+      interp_sact (sigma:=sigma) vvs a v.
+  Proof.
+    induction fuel; simpl; intros; eauto. easy.
+    unfold opt_bind in H; repeat destr_in H; inv H.
+    - econstructor; eauto.
+    - econstructor; eauto.
+    - econstructor; eauto.
+    - econstructor; eauto.
+    - econstructor; eauto.
+    - econstructor; eauto.
+    - econstructor; eauto.
+  Qed.
+  
+  Lemma do_eval_sact_interp_sact:
+    forall vvs a v,
+      do_eval_sact vvs a = Some v ->
+      interp_sact (sigma:=sigma) vvs a v.
+  Proof.
+    intros; eapply eval_sact_interp_sact; eauto.
+  Qed.
+
+  Fixpoint eval_sact_no_vars (a: sact) : option val :=
+    match a with
+    | SConst v => Some v
+    | SVar v => None
+    | SIf c t f =>
+        let/opt v := eval_sact_no_vars c in
+        match v with
+        | Bits 1 [b] =>
+            if b then eval_sact_no_vars t
+            else eval_sact_no_vars f
+        | _ => None
+        end
+    | SUnop ufn a =>
+        let/opt v := eval_sact_no_vars a in
+        sigma1 ufn v
+    | SBinop ufn a1 a2 =>
+        let/opt v1 := eval_sact_no_vars a1 in
+        let/opt v2 := eval_sact_no_vars a2 in
+        sigma2 ufn v1 v2
+    | SExternalCall ufn a =>
+        let/opt v := eval_sact_no_vars a in
+        Some (sigma ufn v)
+    end.
+  
+  Lemma list_assoc_filter:
+    forall {K V: Type} {eqdec: EqDec K} (l: list (K*V)) f k,
+      (forall v, f (k,v) = true) ->
+      list_assoc l k = list_assoc (filter f l) k.
+  Proof.
+    induction l; simpl; intros; eauto.
+    repeat destr.
+    - subst. simpl. rewrite eq_dec_refl. reflexivity.
+    - subst. simpl. destr. eauto.
+    - eauto.
+  Qed.
+  
+  Lemma interp_sact_same_below:
+    forall vvs1 vvs2 a res n (VSV: vvs_smaller_variables vvs1),
+      (forall v, var_in_sact a v -> v < n) ->
+      (forall x, x < n -> list_assoc vvs1 x = list_assoc vvs2 x) ->
+      interp_sact (sigma:=sigma) vvs1 a res -> interp_sact (sigma:=sigma) vvs2 a res.
+  Proof.
+    induction 4; simpl; intros; eauto.
+    - assert (var < n). apply H. constructor.
+      econstructor; eauto. erewrite <- H0; eauto.
+      apply IHinterp_sact. intros; eapply VSV in H1. apply H1 in H4. red in H4. lia.
+    - constructor.
+    - econstructor. eapply IHinterp_sact1. intros; eapply H; eapply var_in_if_cond; eauto.
+      eapply IHinterp_sact2. intros; eapply H.
+      destr_in H1. eapply var_in_if_true; eauto. eapply var_in_if_false; eauto.
+    - econstructor. eapply IHinterp_sact. intros; eapply H; eapply var_in_sact_unop; eauto. auto.
+    - econstructor. eapply IHinterp_sact1. intros; eapply H; eapply var_in_sact_binop_1; eauto.
+      eapply IHinterp_sact2. intros; eapply H; eapply var_in_sact_binop_2; eauto. auto.
+    - econstructor. eapply IHinterp_sact. intros; eapply H; eapply var_in_sact_external; eauto.
+  Qed.
+
+  Lemma map_filter:
+    forall {A: Type} (f: A -> A) g,
+      (forall x, g x = g (f x)) ->
+      forall l,
+        map f (filter g l) = filter g (map f l).
+  Proof.
+    induction l; simpl; intros; eauto.
+    rewrite <- H. destruct (g a). simpl. congruence. auto.
+  Qed.
+
+  Lemma list_assoc_map:
+    forall {K V: Type} {eqdec: EqDec K} (f: K*V -> K*V) (g: V -> V)
+           (F: forall k1 v1, f (k1,v1) = (k1, g v1))
+           l k,
+      list_assoc (map f l) k = option_map g (list_assoc l k).
+  Proof.
+    induction l; simpl; intros; eauto.
+    destruct a. rewrite F. destr. subst. simpl. reflexivity.
+  Qed.
+  
+  Lemma interp_sact_replace:
+    forall vvs var v' ,
+      interp_sact (sigma:=sigma) vvs (SVar var) v' ->
+      forall a res,
+        interp_sact (sigma:=sigma) vvs a res ->
+        interp_sact (sigma:=sigma) vvs (replace_all_occurrences_in_sact a var v') res.
+  Proof.
+    induction 2; simpl; intros; eauto.
+    - destr.
+      + subst. inv H. rewrite H0 in H3. inv H3.
+        exploit (interp_sact_determ (ext_fn_t:=ext_fn_t) (sigma:=sigma)). apply H1. apply H4.
+        intros ->; econstructor.
+      + econstructor; eauto.
+    - econstructor.
+    - econstructor; eauto.
+      destruct b; eauto.
+    - econstructor; eauto.
+    - econstructor; eauto.
+    - econstructor; eauto.
+  Qed.
+
+  Lemma interp_sact_replace_inv:
+    forall vvs (VSV: vvs_smaller_variables vvs) var v' ,
+      interp_sact (sigma:=sigma) vvs (SVar var) v' ->
+      forall a n (BELOW: forall v, var_in_sact a v -> v < n) res,
+        interp_sact (sigma:=sigma) vvs (replace_all_occurrences_in_sact a var v') res ->
+        interp_sact (sigma:=sigma) vvs a res.
+  Proof.
+    intros vvs VSV var v' INTvar a n.
+    change n with (projT1 (existT (fun _ => sact) n a)).
+    change a with (projT2 (existT (fun _ => sact) n a)) at 1 3 4.
+    generalize (existT (fun _ => sact) n a).
+    clear n a. intro s. pattern s.
+    eapply well_founded_induction.
+    apply wf_order_sact. clear s.
+    intros (n1 & a) IH. simpl.
+    intros BELOW res INTres.
+    destruct a; simpl in *.
+    - destr_in INTres.
+      + subst. inv INTres. eauto.
+      + eauto.
+    - inv INTres; econstructor.
+    - inv INTres.
+      econstructor.
+      eapply (IH (existT _ n1 a1)); eauto. constructor 2. simpl; lia.
+      simpl; intros. eapply BELOW. eapply var_in_if_cond; eauto.
+      eapply (IH (existT _ n1 (if b then a2 else a3))); eauto. constructor 2. destruct b; simpl; lia.
+      simpl; intros. eapply BELOW. destruct b.
+      eapply var_in_if_true; eauto. eapply var_in_if_false; eauto. simpl.
+      destruct b; eauto.
+    - inv INTres; econstructor; eauto.
+      eapply (IH (existT _ n1 a)); eauto. constructor 2. simpl; lia.
+      simpl; intros. eapply BELOW. eapply var_in_sact_unop; eauto.
+    - inv INTres; econstructor; eauto.
+      eapply (IH (existT _ n1 a1)); eauto. constructor 2. simpl; lia.
+      simpl; intros. eapply BELOW. eapply var_in_sact_binop_1; eauto.
+      eapply (IH (existT _ n1 a2)); eauto. constructor 2. simpl; lia.
+      simpl; intros. eapply BELOW. eapply var_in_sact_binop_2; eauto.
+    - inv INTres; econstructor; eauto.
+      eapply (IH (existT _ n1 a)); eauto. constructor 2. simpl; lia.
+      simpl; intros. eapply BELOW. eapply var_in_sact_external; eauto.
+  Qed.
+
+  Lemma interp_sact_replace_iff:
+    forall vvs (VSV: vvs_smaller_variables vvs) var v' ,
+      interp_sact (sigma:=sigma) vvs (SVar var) v' ->
+      forall a t (WT: wt_sact (Sigma:=Sigma) vvs a t) res,
+        interp_sact (sigma:=sigma) vvs (replace_all_occurrences_in_sact a var v') res <->
+        interp_sact (sigma:=sigma) vvs a res.
+  Proof.
+    split; intros.
+    - eapply interp_sact_replace_inv; eauto.
+      eapply wt_sact_valid_vars. 2: eauto.
+      apply vvs_range_max_var.
+    - eapply interp_sact_replace; eauto.
+  Qed.
+
+  Lemma interp_sact_replace_one_variable:
+    forall vvs (VSV: vvs_smaller_variables vvs) var v' ,
+      interp_sact (sigma:=sigma) vvs (SVar var) v' ->
+      forall a n,
+        (forall v, var_in_sact a v -> v < n) ->
+        forall res,
+          interp_sact (sigma:=sigma) vvs a res ->
+          interp_sact (sigma:=sigma)
+                      (replace_all_occurrences_in_vars
+                         (filter (fun '(n, _) => negb (beq_dec n var)) vvs) var v')
+                      (replace_all_occurrences_in_sact a var v') res.
+  Proof.
+    intros vvs VSV var v' INTvar.
+    intros a n.
+    change n with (projT1 (existT (fun _ => sact) n a)).
+    change a with (projT2 (existT (fun _ => sact) n a)) at 1 3 4.
+    generalize (existT (fun _ => sact) n a).
+    clear n a. intro s. pattern s.
+    eapply well_founded_induction.
+    apply wf_order_sact. clear s.
+    intros (n1 & a) IH. simpl.
+    intros BELOW res INTres.
+    inv INTres; simpl.
+    - destr.
+      + subst. inv INTvar. rewrite H2 in H. inv H.
+        exploit (interp_sact_determ (sigma:=sigma) (ext_fn_t:=ext_fn_t)).
+        apply H3. apply H0. intros; subst. constructor.
+      + econstructor. unfold replace_all_occurrences_in_vars.
+        rewrite list_assoc_map with (g:=fun '(t,a) => (t, replace_all_occurrences_in_sact a var v')).
+        rewrite <- list_assoc_filter.
+        2: intros; rewrite negb_true_iff, beq_dec_false_iff; auto.
+        2: intros; repeat destr; eauto.
+        setoid_rewrite H. simpl. eauto.
+        eapply (IH (existT _ var0 a0)).
+        constructor. eapply BELOW. constructor.
+        simpl. intros; eapply VSV; eauto.
+        simpl. auto.
+    - constructor.
+    - econstructor.
+      eapply (IH (existT _ n1 c)). constructor 2. simpl; lia.
+      simpl. intros; eapply BELOW. apply var_in_if_cond; eauto. simpl. eauto.
+      trim (IH (existT _ n1 (if b then t else f))). constructor 2. destruct b; simpl; lia.
+      simpl in IH.
+      trim IH. intros; eapply BELOW.
+      destruct b. eapply var_in_if_true; eauto. eapply var_in_if_false; eauto.
+      specialize (IH _ H0).
+      destr; eauto.
+    - econstructor.
+      eapply (IH (existT _ n1 a0)). constructor 2. simpl; lia.
+      simpl. intros; eapply BELOW. apply var_in_sact_unop; eauto. simpl. eauto.
+      auto.
+    - econstructor.
+      eapply (IH (existT _ n1 a1)). constructor 2. simpl; lia.
+      simpl. intros; eapply BELOW. apply var_in_sact_binop_1; eauto. simpl. eauto.
+      eapply (IH (existT _ n1 a2)). constructor 2. simpl; lia.
+      simpl. intros; eapply BELOW. apply var_in_sact_binop_2; eauto. simpl. eauto. auto.
+    - econstructor.
+      eapply (IH (existT _ n1 a0)). constructor 2. simpl; lia.
+      simpl. intros; eapply BELOW. apply var_in_sact_external; eauto. simpl. eauto.
+  Qed.
+
+  Lemma interp_sact_replace_one:
+    forall vvs (VSV: vvs_smaller_variables vvs) var v' ,
+      interp_sact (sigma:=sigma) vvs (SVar var) v' ->
+      forall a n,
+        (forall v, var_in_sact a v -> v < n) ->
+        forall res,
+          interp_sact (sigma:=sigma) vvs a res ->
+          interp_sact (sigma:=sigma)
+                      (replace_all_occurrences_in_vars vvs var v')
+                      (replace_all_occurrences_in_sact a var v') res.
+  Proof.
+    intros vvs VSV var v' INTvar.
+    intros a n.
+    change n with (projT1 (existT (fun _ => sact) n a)).
+    change a with (projT2 (existT (fun _ => sact) n a)) at 1 3 4.
+    generalize (existT (fun _ => sact) n a).
+    clear n a. intro s. pattern s.
+    eapply well_founded_induction.
+    apply wf_order_sact. clear s.
+    intros (n1 & a) IH. simpl.
+    intros BELOW res INTres.
+    inv INTres; simpl.
+    - destr.
+      + subst. inv INTvar. rewrite H2 in H. inv H.
+        exploit (interp_sact_determ (sigma:=sigma) (ext_fn_t:=ext_fn_t)).
+        apply H3. apply H0. intros; subst. constructor.
+      + econstructor. unfold replace_all_occurrences_in_vars.
+        rewrite list_assoc_map with (g:=fun '(t,a) => (t, replace_all_occurrences_in_sact a var v')).
+        2: intros; repeat destr; eauto.
+        setoid_rewrite H. simpl. eauto.
+        eapply (IH (existT _ var0 a0)).
+        constructor. eapply BELOW. constructor.
+        simpl. intros; eapply VSV; eauto.
+        simpl. auto.
+    - constructor.
+    - econstructor.
+      eapply (IH (existT _ n1 c)). constructor 2. simpl; lia.
+      simpl. intros; eapply BELOW. apply var_in_if_cond; eauto. simpl. eauto.
+      trim (IH (existT _ n1 (if b then t else f))). constructor 2. destruct b; simpl; lia.
+      simpl in IH.
+      trim IH. intros; eapply BELOW.
+      destruct b. eapply var_in_if_true; eauto. eapply var_in_if_false; eauto.
+      specialize (IH _ H0).
+      destr; eauto.
+    - econstructor.
+      eapply (IH (existT _ n1 a0)). constructor 2. simpl; lia.
+      simpl. intros; eapply BELOW. apply var_in_sact_unop; eauto. simpl. eauto.
+      auto.
+    - econstructor.
+      eapply (IH (existT _ n1 a1)). constructor 2. simpl; lia.
+      simpl. intros; eapply BELOW. apply var_in_sact_binop_1; eauto. simpl. eauto.
+      eapply (IH (existT _ n1 a2)). constructor 2. simpl; lia.
+      simpl. intros; eapply BELOW. apply var_in_sact_binop_2; eauto. simpl. eauto. auto.
+    - econstructor.
+      eapply (IH (existT _ n1 a0)). constructor 2. simpl; lia.
+      simpl. intros; eapply BELOW. apply var_in_sact_external; eauto. simpl. eauto.
+  Qed.
+  
+  Lemma interp_eval:
+    forall vvs vvs' a b
+           (VSV1: vvs_smaller_variables vvs)
+           (VSV2: vvs_smaller_variables vvs') ta tb
+           (WTa: wt_sact (Sigma:=Sigma) vvs a ta)
+           (WTb: wt_sact (Sigma:=Sigma) vvs' b tb)
+    ,
+      (exists m, forall n, n >= m ->
+                           eval_sact vvs a n = eval_sact vvs' b n) ->
+      (forall res, interp_sact (sigma:=sigma) vvs a res -> interp_sact (sigma:=sigma) vvs' b res).
+  Proof.
+    intros.
+    destruct H.
+    eapply interp_sact_eval_sact in H0; eauto.
+    eapply eval_sact_more_fuel with (n2:=max x _) in H0.
+    2: apply Nat.le_max_r.
+    rewrite H in H0. 2: lia.
+    eapply eval_sact_interp_sact; eauto.
+  Qed.
+
+  Lemma interp_eval_iff:
+    forall vvs vvs' a b
+           (VSV1: vvs_smaller_variables vvs)
+           (VSV2: vvs_smaller_variables vvs') ta tb
+           (WTa: wt_sact (Sigma:=Sigma) vvs a ta)
+           (WTb: wt_sact (Sigma:=Sigma) vvs' b tb)
+    ,
+      (exists m, forall n, n >= m ->
+                           eval_sact vvs a n = eval_sact vvs' b n) ->
+      (forall res, interp_sact (sigma:=sigma) vvs a res <-> interp_sact (sigma:=sigma) vvs' b res).
+  Proof.
+    intros vvs vvs' a b VSV1 VSV2 ta tb WTa WTb (m & EQ) res.
+    split; intros.
+    - eapply interp_eval. 6: eauto. all: eauto.
+    - eapply interp_eval. 6: eauto. all: eauto.
+      exists m; intros; eauto. rewrite EQ; auto.
+  Qed.
+
+  Lemma eval_sact_no_vars_interp:
+    forall vvs s v
+           (EVAL: eval_sact_no_vars s = Some v),
+      interp_sact (sigma:=sigma) vvs s v.
+  Proof.
+    induction s; simpl; intros; eauto; unfold opt_bind in EVAL; repeat destr_in EVAL; inv EVAL.
+    - econstructor; eauto.
+    - econstructor; eauto.
+    - econstructor; eauto.
+    - econstructor; eauto.
+    - econstructor; eauto.
+    - econstructor; eauto.
+  Qed.
+
+  Context {wt_sigma: forall ufn vc,
+      wt_val (arg1Sig (Sigma ufn)) vc ->
+      wt_val (retSig (Sigma ufn)) (sigma ufn vc)}.
+
+  Lemma var_in_sact_replace:
+    forall a n v x,
+      var_in_sact (replace_all_occurrences_in_sact a n v) x ->
+      var_in_sact a x.
+  Proof.
+    induction a; simpl; intros; eauto.
+    - destr_in H; inv H. constructor.
+    - inv H. eapply var_in_if_cond; eauto.
+      eapply var_in_if_true; eauto.
+      eapply var_in_if_false; eauto.
+    - inv H. eapply var_in_sact_unop; eauto.
+    - inv H. eapply var_in_sact_binop_1; eauto.
+      eapply var_in_sact_binop_2; eauto.
+    - inv H. eapply var_in_sact_external; eauto.
+  Qed.
+
+  Lemma vvs_smaller_variables_replace:
+    forall vvs n v,
+      vvs_smaller_variables vvs ->
+      vvs_smaller_variables (replace_all_occurrences_in_vars vvs n v).
+  Proof.
+    unfold vvs_smaller_variables; intros.
+    setoid_rewrite list_assoc_map with (g:= fun '(t,a) => (t, replace_all_occurrences_in_sact a n v)) in H0.
+    2: intros; repeat destr.
+    unfold option_map in H0; repeat destr_in H0; inv H0.
+    eapply var_in_sact_replace in H1; eauto.
+  Qed.
+
+  Lemma wt_sact_replace:
+    forall vvs a t n v t1,
+      wt_sact (Sigma:=Sigma) vvs a t ->
+      wt_sact (Sigma:=Sigma) vvs (SVar n) t1 ->
+      wt_val t1 v ->
+      wt_sact (Sigma:=Sigma) vvs (replace_all_occurrences_in_sact a n v) t.
+  Proof.
+    induction 1; simpl; intros; eauto.
+    - destr.
+      + subst. inv H0. rewrite H in H3; inv H3. econstructor; eauto.
+      + econstructor. eauto.
+    - inv H0. econstructor. eauto.
+    - econstructor; eauto.
+    - econstructor; eauto.
+    - econstructor; eauto.
+    - econstructor; eauto.
+  Qed.
+
+  Lemma wt_sact_replace_vars:
+    forall vvs a t n v t1,
+      wt_sact (Sigma:=Sigma) vvs a t ->
+      wt_sact (Sigma:=Sigma) vvs (SVar n) t1 ->
+      wt_val t1 v ->
+      wt_sact (Sigma:=Sigma) (replace_all_occurrences_in_vars vvs n v) (replace_all_occurrences_in_sact a n v) t.
+  Proof.
+    induction 1; simpl; intros; eauto.
+    - destr.
+      + subst. inv H0. rewrite H in H3; inv H3. econstructor; eauto.
+      + econstructor.
+        setoid_rewrite list_assoc_map with (g:= fun '(t,a) => (t, replace_all_occurrences_in_sact a n v)). setoid_rewrite H. simpl; eauto. intros; repeat destr.
+    - inv H0. econstructor. eauto.
+    - econstructor; eauto.
+    - econstructor; eauto.
+    - econstructor; eauto.
+    - econstructor; eauto.
+  Qed.
+
+  Lemma wt_sact_replace_vars':
+    forall vvs a t n v t1,
+      wt_sact (Sigma:=Sigma) vvs a t ->
+      wt_sact (Sigma:=Sigma) vvs (SVar n) t1 ->
+      wt_val t1 v ->
+      wt_sact (Sigma:=Sigma) (replace_all_occurrences_in_vars vvs n v) a t.
+  Proof.
+    induction 1; simpl; intros; eauto.
+    - econstructor.
+      setoid_rewrite list_assoc_map with (g:= fun '(t,a) => (t, replace_all_occurrences_in_sact a n v)).
+      setoid_rewrite H. simpl; eauto. intros; repeat destr.
+    - inv H0. econstructor. eauto.
+    - econstructor; eauto.
+    - econstructor; eauto.
+    - econstructor; eauto.
+    - econstructor; eauto.
+  Qed.
+
+  Lemma wt_vvs_replace:
+    forall vvs n v t1,
+      wt_vvs (Sigma:=Sigma) vvs ->
+      wt_sact (Sigma:=Sigma) vvs (SVar n) t1 ->
+      wt_val t1 v ->
+      wt_vvs (Sigma:=Sigma) (replace_all_occurrences_in_vars vvs n v).
+  Proof.
+    unfold wt_vvs; intros.
+    setoid_rewrite list_assoc_map with (g:= fun '(t,a) => (t, replace_all_occurrences_in_sact a n v)) in H2.
+    2: intros; repeat destr.
+    unfold option_map in H2; repeat destr_in H2; inv H2.
+    eapply wt_sact_replace_vars; eauto.
+  Qed.
+
+  Lemma eval_sact_no_vars_wt:
+    forall vvs s t
+           (WT: wt_sact (Sigma:=Sigma) vvs s t)
+           v
+           (EVAL: eval_sact_no_vars s = Some v),
+      wt_val t v.
+  Proof.
+    induction 1; simpl; intros; unfold opt_bind in EVAL; repeat destr_in EVAL; inv EVAL;
+      try now (eauto).
+    eapply Wt.wt_unop_sigma1; eauto.
+    eapply Wt.wt_binop_sigma1; eauto.
+  Qed.
+
+  Definition simplify_var (sf: simple_form) var :=
+    match list_assoc (vars sf) var with
+      Some (t, a) =>
+           match eval_sact_no_vars a with
+             Some v => (replace_all_occurrences sf var v, [(var,v)])
+           | None => (sf, [])
+           end
+    | _ => (sf, [])
+    end.
+
+  Lemma var_not_in_sact_replace:
+    forall s0 v0 v,
+      ~ var_in_sact (replace_all_occurrences_in_sact s0 v0 v) v0.
+  Proof.
+    induction s0; simpl; intros; eauto.
+    - destr; inversion 1. congruence.
+    - inversion 1.
+    - inversion 1; subst; intuition eauto.
+    - inversion 1; subst; intuition eauto.
+    - inversion 1; subst; intuition eauto.
+    - inversion 1; subst; intuition eauto.
+  Qed.
+
+  Lemma simplify_var_correct:
+    forall sf var sf' l
+           (SIMP: simplify_var sf var = (sf', l))
+           (VSV: vvs_smaller_variables (vars sf))
+           (WT: wt_vvs (Sigma:=Sigma) (vars sf)),
+      Forall (fun '(var,v) => interp_sact (sigma:=sigma) (vars sf') (SVar var) v) l
+      /\ vvs_smaller_variables (vars sf')
+      /\ wt_vvs (Sigma:=Sigma) (vars sf')
+      /\ (forall a res t,
+             wt_sact (Sigma:=Sigma) (vars sf) a t ->
+             interp_sact (sigma:=sigma) (vars sf) a res ->
+             interp_sact (sigma:=sigma) (vars sf') a res)
+  /\ (forall x t y res,
+              list_assoc (vars sf) x = Some (t,y) ->
+              interp_sact (sigma:=sigma) (vars sf) y res ->
+              (exists y' ,
+                  list_assoc (vars sf') x = Some (t,y') /\
+                    interp_sact (sigma:=sigma) (vars sf') y' res)
+     ) /\
+  (forall x t y v, list_assoc (vars sf') x = Some (t,y) ->
+                   var_in_sact y v -> ~ In v (map fst l)) /\
+        (forall x t y,
+            list_assoc (vars sf') x = Some (t, y) ->
+            exists y' ,
+              list_assoc (vars sf) x = Some (t, y') /\
+                forall v, var_in_sact y v -> var_in_sact y' v).
+  Proof.
+    unfold simplify_var. intros. repeat destr_in SIMP; inv SIMP; eauto.
+    assert (VSV': vvs_smaller_variables (vars (replace_all_occurrences sf var v))).
+    eapply vvs_smaller_variables_replace; now eauto.
+    assert (WTVVS':  wt_vvs (Sigma:=Sigma) (vars (replace_all_occurrences sf var v))).
+    {
+      eapply wt_vvs_replace; eauto.
+      econstructor. eauto.
+      eapply eval_sact_no_vars_wt; eauto.
+    }
+    repeat refine (conj _ _); eauto.
+    - repeat constructor.
+      simpl.
+      erewrite <- interp_sact_replace_iff; eauto.
+      eapply interp_sact_replace_one; eauto.
+      + econstructor. eauto. eapply eval_sact_no_vars_interp; eauto.
+      + intros. eapply wt_sact_valid_vars. 3: eauto. 2: econstructor; eauto.
+        apply vvs_range_max_var.
+      + econstructor. eauto.
+        eapply eval_sact_no_vars_interp; eauto.
+      + econstructor.
+        setoid_rewrite list_assoc_map with (g:= fun '(t,a) => (t, replace_all_occurrences_in_sact a var v)).
+        setoid_rewrite Heqo. simpl; eauto.
+        intros; repeat destr.
+        eapply interp_sact_replace_one. eauto.
+        econstructor. eauto.
+        eapply eval_sact_no_vars_interp; eauto.
+        eapply wt_sact_valid_vars. 2: eapply (WT var). apply vvs_range_max_var.
+        eauto.
+        eapply eval_sact_no_vars_interp; eauto.
+      + econstructor.
+        setoid_rewrite list_assoc_map with (g:= fun '(t,a) => (t, replace_all_occurrences_in_sact a var v)).
+        setoid_rewrite Heqo. simpl; eauto.
+        intros; repeat destr.
+        Unshelve. exact Sigma.
+    - simpl. intros.
+      erewrite <- interp_sact_replace_iff; eauto.
+      eapply interp_sact_replace_one; eauto.
+      + econstructor. eauto. eapply eval_sact_no_vars_interp; eauto.
+      + intros. eapply wt_sact_valid_vars. 3: eauto. 2: eauto.
+        apply vvs_range_max_var.
+      + econstructor.
+        setoid_rewrite list_assoc_map with (g:= fun '(t,a) => (t, replace_all_occurrences_in_sact a var v)).
+        setoid_rewrite Heqo. simpl; eauto.
+        intros; repeat destr.
+        eapply interp_sact_replace_one. eauto.
+        econstructor. eauto.
+        eapply eval_sact_no_vars_interp; eauto.
+        eapply wt_sact_valid_vars. 2: eapply (WT var). apply vvs_range_max_var.
+        eauto.
+        eapply eval_sact_no_vars_interp; eauto.
+      + eapply wt_sact_replace_vars'. eauto. econstructor; eauto.
+        eapply eval_sact_no_vars_wt; eauto.
+    - simpl. intros.
+      setoid_rewrite list_assoc_map with (g:= fun '(t,a) => (t, replace_all_occurrences_in_sact a var v)).
+      setoid_rewrite H. simpl; eauto.
+      eexists; split; eauto.
+      eapply interp_sact_replace_one; eauto.
+      + econstructor. eauto. eapply eval_sact_no_vars_interp; eauto.
+      + intros. eapply wt_sact_valid_vars. 3: eauto. 2: eauto.
+        apply vvs_range_max_var.
+      + intros; repeat destr.
+    - simpl.
+      setoid_rewrite list_assoc_map with (g:= fun '(t,a) => (t, replace_all_occurrences_in_sact a var v)). 2: intros; destr.
+      unfold option_map; intros x t0 y v0 OM; repeat destr_in OM; inv OM.
+      intros VIS [EQ|[]]. subst.
+
+      eapply var_not_in_sact_replace; eauto.
+    - simpl. intros x t0 y.
+      setoid_rewrite list_assoc_map with (g:= fun '(t,a) => (t, replace_all_occurrences_in_sact a var v)). 2: intros; destr.
+      unfold option_map; intros OM; repeat destr_in OM; inv OM.
+      setoid_rewrite Heqo1. eexists; split; eauto.
+      eapply var_in_sact_replace; eauto.
+    - repeat refine (conj _ _); eauto.
+    - repeat refine (conj _ _); eauto.
+  Qed.
+
+
+  Lemma eval_sact_no_vars_succeeds:
+    forall a (NoVars: forall v, ~ var_in_sact a v)
+           vvs t (WTa: wt_sact (Sigma:=Sigma) vvs a t),
+    exists r, eval_sact_no_vars a = Some r.
+  Proof.
+    induction a; simpl; intros; eauto.
+    - elim (NoVars var). constructor.
+    - inv WTa.
+      edestruct IHa1 as (r1 & EQ1); eauto.
+      intros v VIS; eapply NoVars; eauto. apply var_in_if_cond; eauto.
+      rewrite EQ1. simpl.
+      exploit eval_sact_no_vars_wt. 2: eauto. eauto. intro WTc.
+      apply wt_val_bool in WTc. destruct WTc; subst.
+      destr. eapply IHa2; eauto.
+      intros v VIS; eapply NoVars; eauto. apply var_in_if_true; eauto.
+      eapply IHa3; eauto.
+      intros v VIS; eapply NoVars; eauto. apply var_in_if_false; eauto.
+    - inv WTa.
+      edestruct IHa as (r1 & EQ1); eauto.
+      intros v VIS; eapply NoVars; eauto. apply var_in_sact_unop; eauto.
+      rewrite EQ1. simpl.
+      eapply wt_unop_interp; eauto.
+      eapply eval_sact_no_vars_wt; eauto.
+    - inv WTa.
+      edestruct IHa1 as (r1 & EQ1); eauto.
+      intros v VIS; eapply NoVars; eauto. apply var_in_sact_binop_1; eauto.
+      rewrite EQ1. simpl.
+      edestruct IHa2 as (r2 & EQ2); eauto.
+      intros v VIS; eapply NoVars; eauto. apply var_in_sact_binop_2; eauto.
+      rewrite EQ2. simpl.
+      eapply wt_binop_interp; eauto.
+      eapply eval_sact_no_vars_wt; eauto.
+      eapply eval_sact_no_vars_wt; eauto.
+    - inv WTa.
+      edestruct IHa as (r1 & EQ1); eauto.
+      intros v VIS; eapply NoVars; eauto. apply var_in_sact_external; eauto.
+      rewrite EQ1. simpl. eauto.
+  Qed.
+
+
+  Lemma simplify_vars_preserves:
+    forall (lvars: list nat) sf l sf' l'
+           (FL: fold_left
+                  (fun '(sf, l) var =>
+                     let '(sf, l1) := simplify_var sf var in
+                     (sf,l1++l)) lvars (sf, l) = (sf', l'))
+           (WTV: wt_vvs (Sigma:=Sigma) (vars sf))
+           (VSV: vvs_smaller_variables (vars sf))
+           (NIV: (forall x t y v, list_assoc (vars sf) x = Some (t,y) ->
+                                  var_in_sact y v -> ~ In v (map fst l))),
+      vvs_smaller_variables (vars sf') /\
+        wt_vvs (Sigma:=Sigma) (vars sf') /\ (incl l l')
+      /\ (forall x t y v, list_assoc (vars sf') x = Some (t,y) ->
+                          var_in_sact y v -> ~ In v (map fst l')).
+  Proof.
+    induction lvars; simpl; intros; eauto.
+    - inv FL. repeat refine (conj _ _); eauto. easy.
+    - repeat destr_in FL.
+      edestruct simplify_var_correct as (INT & VSV2 & WT2 & INTERP2 & INTERP3 & NAV1 & VIS1); eauto.
+      edestruct (IHlvars _ _ _ _ FL) as (VSV3 & WTV3 & INCL & NIV2); auto.
+      intros.
+      specialize (NAV1 _ _ _ _ H H0).
+      rewrite map_app. rewrite in_app_iff. intros [IN|IN]; eauto.
+      edestruct VIS1 as (y' & GET2 & IMPL). apply H.
+      eapply NIV in IN; eauto.
+      split; auto. split; auto. split; auto.
+      apply incl_app_inv in INCL. apply INCL.
+  Qed.
+
+  Lemma simplify_vars_correct:
+    forall (lvars: list nat) sf l sf' l'
+           (FL: fold_left
+                  (fun '(sf, l) var =>
+                     let '(sf, l1) := simplify_var sf var in
+                     (sf,l1++l)) lvars (sf, l) = (sf', l'))
+           (SORTED: Sorted lt lvars)
+           (VARS_EXIST: Forall (fun v => exists a t, list_assoc (vars sf) v = Some (t,a)) lvars)
+           (WTV: wt_vvs (Sigma:=Sigma) (vars sf))
+           (ACC: Forall (fun '(var, v) => interp_sact (sigma:=sigma) (vars sf) (SVar var) v) l)
+           (VSV: vvs_smaller_variables (vars sf))
+           (NOvarsl: forall x t y v,
+               list_assoc (vars sf) x = Some (t,y) ->
+               var_in_sact y v -> ~ In v (map fst l) /\ In v lvars)
+    ,
+      (forall x t y res,
+          list_assoc (vars sf) x = Some (t,y) ->
+          interp_sact (sigma:=sigma) (vars sf) y res ->
+          (exists y' ,
+              list_assoc (vars sf') x = Some (t,y') /\
+                interp_sact (sigma:=sigma) (vars sf') y' res)
+      ) /\
+        vvs_smaller_variables (vars sf') /\
+        wt_vvs (Sigma:=Sigma) (vars sf') /\
+        Forall (fun '(var, v) => interp_sact (sigma:=sigma) (vars sf') (SVar var) v) l' /\
+        (forall x t y v, list_assoc (vars sf') x = Some (t,y) ->
+                         var_in_sact y v -> ~ In v (map fst l'))
+      /\ (incl l l')
+  /\ (forall x, In x lvars -> exists v, In (x, v) l').
+  Proof.
+    induction lvars; simpl; intros; eauto.
+    - inv FL. repeat refine (conj _ _); eauto.
+      intros x t y v GET VIS; eapply NOvarsl in GET; eauto. destruct GET; easy.
+      easy. easy.
+    - repeat destr_in FL.
+      edestruct simplify_var_correct as (INT & VSV2 & WT2 & INTERP2 & INTERP3 & NAV1 & VIS1); eauto.
+      edestruct (IHlvars _ _ _ _ FL) as (LGROWS & VSV3 & WT3 & INTERPl & NAV2 & INCL & INl'); auto.
+      * inv SORTED; auto.
+      * inv VARS_EXIST. rewrite Forall_forall in H2 |- *. intros x IN.
+        specialize (H2 _ IN).
+        destruct H2 as (aa & t & GET).
+        move Heqp at bottom. unfold simplify_var in Heqp.
+        repeat destr_in Heqp; inv Heqp; eauto.
+        simpl. unfold replace_all_occurrences_in_vars.
+        setoid_rewrite list_assoc_map with (g:= fun '(t,a0) => (t, replace_all_occurrences_in_sact a0 a v)). 2: intros; destr.
+        setoid_rewrite GET. simpl. do 2 eexists; eauto.
+      * eapply Forall_app. split. eauto.
+        rewrite Forall_forall in ACC |- *. intros (var & v) IN.
+        specialize (ACC _ IN). simpl in ACC.
+        inv ACC. 
+        eapply INTERP2. econstructor; eauto. econstructor; eauto.
+      * intros x t y v GET VIS.
+        split.
+        -- intro IN. rewrite map_app in IN. rewrite in_app_iff in IN.
+           destruct IN; eauto. eapply NAV1; eauto.
+           edestruct VIS1 as (y' & GET2 & IMPL). eauto.
+           apply IMPL in VIS.
+           eapply NOvarsl; eauto.
+        -- edestruct (VIS1 _ _ _ GET) as (y'& GET' & VISS).
+           destruct (NOvarsl _ _ _ _ GET' (VISS _ VIS)) as (? & [EQ|IN]); eauto.
+           exfalso. subst.
+           move Heqp at bottom. unfold simplify_var in Heqp. inv VARS_EXIST.
+           destruct H2 as (? & ? & GETv). rewrite GETv in Heqp.
+           assert (forall x, ~ var_in_sact x0 x).
+           {
+             intros xx VVIS.
+             generalize (VSV v _ _ GETv _ VVIS). intro LT. red in LT.
+             destruct (NOvarsl _ _ _ xx GETv VVIS) as (_ & [EQ|IN]).
+             lia.
+             move SORTED at bottom.
+             apply Sorted_StronglySorted in SORTED.
+             2:{
+               red. intros; lia.
+             }
+             inv SORTED.
+             rewrite Forall_forall in H4; apply H4 in IN; lia.
+           }
+           edestruct (eval_sact_no_vars_succeeds _ H0) as (rr & ESNV). eapply WTV. eauto.
+           rewrite ESNV in Heqp. inv Heqp.
+           revert GET. simpl. unfold replace_all_occurrences_in_vars.
+           setoid_rewrite list_assoc_map with (g:= fun '(t,a0) => (t, replace_all_occurrences_in_sact a0 v rr)). 2: intros; now destr.
+           setoid_rewrite GET'. simpl. intro A; inv A.
+           apply var_not_in_sact_replace in VIS. auto.
+
+      * repeat refine (conj _ _); eauto.
+        intros x t y res GET INTy.
+        edestruct (INTERP3) as (y' & GET2 & INT2); eauto.
+        apply incl_app_inv in INCL. apply INCL.
+        intros x [EQ|IN]; eauto.
+        subst.
+        move Heqp at bottom. unfold simplify_var in Heqp.
+        inv VARS_EXIST.
+        destruct H1 as (? & ? & GETv). rewrite GETv in Heqp.
+        assert (forall x, ~ var_in_sact x0 x).
+        {
+          intros xx VVIS.
+          generalize (VSV _ _ _ GETv _ VVIS). intro LT. red in LT.
+          destruct (NOvarsl _ _ _ xx GETv VVIS) as (_ & [EQ|IN]).
+          lia.
+          move SORTED at bottom.
+          apply Sorted_StronglySorted in SORTED.
+          2:{
+            red. intros; lia.
+          }
+          inv SORTED.
+          rewrite Forall_forall in H3; apply H3 in IN; lia.
+        }
+        edestruct (eval_sact_no_vars_succeeds _ H) as (rr & ESNV). eapply WTV. eauto.
+        rewrite ESNV in Heqp. inv Heqp.
+        exists rr. eapply INCL. simpl. left. auto.
+  Qed.
+
+  Lemma list_assoc_filter2:
+    forall {K V: Type} {eqdec: EqDec K} (l: list (K*V)) name k,
+      list_assoc (filter (fun '(n,_) => negb (beq_dec n name)) l) k =
+        if beq_dec k name then None else list_assoc l k.
+  Proof.
+    induction l; simpl; intros; eauto.
+    repeat destr.
+    destruct a.
+    destruct (beq_dec k0 name) eqn:?; simpl. apply beq_dec_iff in Heqb. subst.
+    rewrite IHl. destr. destr. subst. apply beq_dec_false_iff in Heqb. congruence.
+    destr. subst. rewrite Heqb. auto. eauto.
+  Qed.
+
+  Lemma wt_sact_remove_one:
+    forall vvs v
+           (NV: forall x t y, list_assoc vvs x = Some (t,y) -> ~ var_in_sact y v)
+           a t
+           (WTa: wt_sact (Sigma:=Sigma) vvs a t)
+           (NVa: ~ var_in_sact a v),
+      wt_sact (Sigma:=Sigma) (filter (fun '(n, _) => negb (beq_dec n v)) vvs) a t.
+  Proof.
+    induction 2; simpl; intros; eauto.
+    - econstructor; eauto.
+      rewrite <- list_assoc_filter. eauto.
+      intros. rewrite negb_true_iff, beq_dec_false_iff; auto.
+      intro; subst. apply NVa. constructor.
+    - econstructor; eauto.
+    - econstructor; eauto.
+      apply IHWTa1. intro VIS; apply NVa; apply var_in_if_cond; auto.
+      apply IHWTa2. intro VIS; apply NVa; apply var_in_if_true; auto.
+      apply IHWTa3. intro VIS; apply NVa; apply var_in_if_false; auto.
+    - econstructor; eauto.
+      apply IHWTa. intro VIS; apply NVa; apply var_in_sact_unop; auto.
+    - econstructor; eauto.
+      apply IHWTa1. intro VIS; apply NVa; apply var_in_sact_binop_1; auto.
+      apply IHWTa2. intro VIS; apply NVa; apply var_in_sact_binop_2; auto.
+    - econstructor; eauto.
+      apply IHWTa. intro VIS; apply NVa; apply var_in_sact_external; auto.
+  Qed.
+
+  Lemma eval_sact_bound:
+    forall vvs : var_value_map,
+      vvs_smaller_variables vvs ->
+      forall (a : SimpleForm.sact) t (WTa: wt_sact (Sigma:=Sigma) vvs a t),
+        let bnd := (S (max_var vvs) + vvs_size vvs (S (max_var vvs)) + size_sact a) in
+        forall m, m >= bnd ->
+        eval_sact vvs a m = None ->
+        forall n, n >= m -> eval_sact vvs a n = None.
+  Proof.
+    intros.
+    destruct (eval_sact vvs a n) eqn:?; auto.
+    eapply eval_sact_interp_sact in Heqo.
+    eapply interp_sact_eval_sact in Heqo; eauto.
+    eapply eval_sact_more_fuel with (n2:= m) in Heqo. congruence. unfold bnd in H0. lia.
+  Qed.
+
+  Lemma remove_var_correct:
+    forall vvs (VSV: vvs_smaller_variables vvs) (* (WTvvs: wt_vvs (Sigma:=Sigma) vvs) *) v
+           (NV: forall x t y, list_assoc vvs x = Some (t,y) -> ~ var_in_sact y v)
+           a
+           t (WTa: wt_sact (Sigma:=Sigma) vvs a t)
+           (NVa: ~ var_in_sact a v) res,
+      interp_sact (sigma:=sigma) vvs a res <->
+        interp_sact (sigma:=sigma) (filter (fun '(n,_) => negb (beq_dec n v)) vvs) a res.
+  Proof.
+    intros. eapply interp_eval_iff. eauto.
+    red; intros.
+    generalize (list_assoc_filter2 vvs v v0). rewrite H. destr.
+    rewrite beq_dec_false_iff in Heqb. intros. symmetry in H1. eauto. eauto.
+    eapply wt_sact_remove_one; eauto.
+
+    (* set (F := fun vvs => (S (max_var vvs) + vvs_size vvs (S (max_var vvs)) + size_sact a)). *)
+    (* set (vvs2 := (filter (fun '(n,_) => negb (beq_dec n v)) vvs)). *)
+    (* exists (max (F vvs) (F vvs2)). *)
+    exists O. intros n0 _.
+    intros.
+    clear VSV WTa.
+    revert a NVa. induction n0; simpl; intros; eauto.
+    unfold opt_bind.
+    destr.
+    - rewrite <- list_assoc_filter. repeat destr.  eauto.
+      intros; rewrite negb_true_iff, beq_dec_false_iff; auto.
+      intro; subst. apply NVa. constructor.
+    - rewrite <- IHn0. repeat destr.
+      eapply IHn0. intro VIS; apply NVa; eapply var_in_if_true; auto.
+      eapply IHn0. intro VIS; apply NVa; eapply var_in_if_false; auto.
+      intro VIS; apply NVa; eapply var_in_if_cond; auto.
+    - rewrite <- IHn0. repeat destr.
+      intro VIS; apply NVa; eapply var_in_sact_unop; auto.
+    - rewrite <- ! IHn0. auto.
+      intro VIS; apply NVa; eapply var_in_sact_binop_2; auto.
+      intro VIS; apply NVa; eapply var_in_sact_binop_1; auto.
+    - rewrite <- IHn0. repeat destr.
+      intro VIS; apply NVa; eapply var_in_sact_external; auto.
+  Qed.
+
+  Lemma remove_var_preserves_vsv:
+    forall l sf (VSV: vvs_smaller_variables (vars sf)),
+      vvs_smaller_variables (vars (remove_by_name_var sf l)).
+  Proof.
+    simpl. red; intros.
+    generalize (list_assoc_filter2 (vars sf) l v). rewrite H. destr.
+    rewrite beq_dec_false_iff in Heqb. intros. symmetry in H1. eauto.
+  Qed.
+
+  Lemma remove_vars_preserves_vsv:
+    forall l sf (VSV: vvs_smaller_variables (vars sf)),
+      vvs_smaller_variables (vars (fold_left remove_by_name_var l sf)).
+  Proof.
+    induction l; simpl; intros; eauto.
+    apply IHl. apply remove_var_preserves_vsv. auto.
+  Qed.
+
+  Lemma remove_var_preserves_wt_vvs:
+    forall l sf (WT_VVS: wt_vvs (Sigma:=Sigma) (vars sf))
+           (NV: forall (x : nat) (t0 : type) (y : SimpleForm.sact),
+               list_assoc (vars sf) x = Some (t0, y) -> ~ var_in_sact y l),
+      wt_vvs (Sigma:=Sigma) (vars (remove_by_name_var sf l)).
+  Proof.
+    simpl. red; intros.
+    generalize (list_assoc_filter2 (vars sf) l v). rewrite H. destr.
+    rewrite beq_dec_false_iff in Heqb. intros. symmetry in H0. eauto.
+    eapply wt_sact_remove_one; eauto.
+  Qed.
+
+  Lemma remove_vars_preserves_wt_vvs:
+    forall l sf (WT_VVS: wt_vvs (Sigma:=Sigma) (vars sf))
+           (NV: forall (x : nat) (t0 : type) (y : SimpleForm.sact) v,
+               list_assoc (vars sf) x = Some (t0, y) -> var_in_sact y v -> ~ In v l),
+      wt_vvs (Sigma:=Sigma) (vars (fold_left remove_by_name_var l sf)).
+  Proof.
+    induction l; simpl; intros; eauto.
+    apply IHl.
+    apply remove_var_preserves_wt_vvs; auto.
+    intros x t0 y GET VIS; eapply NV; eauto.
+    simpl.
+    intros x t0 y v GET VIS IN.
+    generalize (list_assoc_filter2 (vars sf) a x). rewrite GET. destr.
+    rewrite beq_dec_false_iff in Heqb. intros. symmetry in H. eapply NV; eauto.
+  Qed.
+
+  Lemma remove_vars_correct:
+    forall l sf (VSV: vvs_smaller_variables (vars sf)) 
+           (NV: forall v x t y, list_assoc (vars sf) x = Some (t,y) -> var_in_sact y v -> ~ In v l)
+           a
+           t (WTa: wt_sact (Sigma:=Sigma) (vars sf) a t)
+           (NVa: forall v, var_in_sact a v -> ~ In v l) res,
+      interp_sact (sigma:=sigma) (vars sf) a res <->
+        interp_sact (sigma:=sigma) (vars (fold_left remove_by_name_var l sf)) a res.
+  Proof.
+    induction l; simpl; intros; eauto. tauto.
+    rewrite <- IHl.
+    - simpl. eapply remove_var_correct; eauto.
+      + intros x t0 y GET VIS; eapply NV; eauto.
+      + intro VIS; eapply NVa; eauto.
+    - eapply remove_var_preserves_vsv; eauto.
+    - simpl. intros.
+      generalize (list_assoc_filter2 (vars sf) a x). rewrite H. destr.
+      rewrite beq_dec_false_iff in Heqb. intros. symmetry in H1. eauto.
+      eapply NV in H1. 2: eauto. intuition.
+    - simpl. eapply wt_sact_remove_one; eauto.
+      + intros x t0 y GET VIS; eapply NV in VIS; eauto.
+      + intro VIS; eapply NVa; eauto.
+    - intros v VIS IN; eapply NVa; eauto.
+  Qed.
+
+  Definition inlining_pass (sf: simple_form)
+    : simple_form * list (nat * val) :=
     (* Try to determine the value of variables *)
-    let (sf', lv) :=
-      fold_left
-        (fun '(sf', l) '(var, ua) =>
-          if negb (contains_vars ua) then
-            match interp_action r sigma [] log_empty log_empty ua with
-            | None => (sf', []) (* Should never happen *)
-            | Some (_, v, _) => (
-               replace_all_occurrences (remove_by_name_var sf' var) var v,
-               (var, v)::l)
-            end
-          else (sf', l))
-        (vars sf) (sf, [])
-    in
-    (* Try to determine the result of extcalls *)
-    fold_left
-      (fun '(sf'', l) '(efn, ei) =>
-        if (negb (contains_vars (econd ei))) then
-          match interp_action r sigma [] log_empty log_empty (econd ei) with
-          | None => (sf'', []) (* Should never happen *)
-          | Some (_, cv, _) =>
-            match cv with
-            | Bits 1 [true] =>
-              if (negb (contains_vars (earg ei))) then
-                match
-                  interp_action r sigma [] log_empty log_empty
-                    (UExternalCall efn (earg ei))
-                with
-                | None => (sf'', l) (* Should nevet_r happen *)
-                | Some (_, r, _) =>
-                  (remove_by_name_extc sf'' (ebind ei), (ebind ei, r)::l)
-                end
-              else (set_cond_true_by_name sf'' (ebind ei), l)
-            | _ => (remove_by_name_extc sf'' (ebind ei), l)
-            end
-          end
-        else (sf'', l))
-      (external_calls sf') (sf', lv).
+    let ks := NatSort.sort (map fst (vars sf)) in
+    let '(sf,l) := fold_left
+                     (fun '(sf,l) var =>
+                        let '(sf,l1) := simplify_var sf var in
+                        (sf, l1++l))
+                     ks (sf,[]) in
+    let sf := fold_left (remove_by_name_var) (map fst l) sf in
+    (sf,l).
+
+  Lemma inlining_pass_preserves:
+    forall sf sf' l
+           (IP: inlining_pass sf = (sf', l))
+           (VSV: vvs_smaller_variables (vars sf))
+           (WT: wt_vvs (Sigma:=Sigma) (vars sf)),
+      vvs_smaller_variables (vars sf') /\ wt_vvs (Sigma:=Sigma) (vars sf').
+  Proof.
+    unfold inlining_pass. intros.
+    repeat destr_in IP. inv IP.
+    exploit simplify_vars_preserves; eauto.
+    intros (VVS' & WT' & _ & NIV).
+    split. eapply remove_vars_preserves_vsv. eauto.
+    eapply remove_vars_preserves_wt_vvs. eauto. eauto.
+  Qed.
+
+  Lemma sorted_lt:
+    forall l,
+      NoDup l ->
+      Sorted lt (NatSort.sort l).
+  Proof.
+    intros.
+    generalize (NatSort.Sorted_sort l). intros.
+
+    Lemma Sorted_strict:
+      forall le1 le2 (STRICT: forall x y, le2 x y <-> (le1 x y /\ x <> y))
+             (l: list nat),
+        Sorted le1 l ->
+        NoDup l ->
+        Sorted le2 l.
+    Proof.
+      induction 2; simpl; intros; eauto.
+      inv H1. econstructor. eauto.
+      inv H0. econstructor. econstructor. rewrite STRICT. split; auto. intro; subst. apply H4; simpl; auto.
+    Qed.
+    eapply Sorted_strict. 2: apply H0.
+    intros. simpl. fold (Nat.leb x y).  unfold is_true. rewrite Nat.leb_le. lia.
+    eapply Permutation.Permutation_NoDup. 2: apply H.
+    apply NatSort.Permuted_sort.
+  Qed.
+
+  Lemma in_list_assoc:
+    forall {K V: Type} {eqdec: EqDec K} (l: list (K*V))
+           (ND: NoDup (map fst l)) k v,
+      In (k,v) l -> list_assoc l k = Some v.
+  Proof.
+    induction l; simpl; intros; eauto. easy.
+    repeat destr; eauto.
+    - subst. destruct H. inv H. auto. simpl in ND. inv ND. elim H2.
+      change k0 with (fst (k0, v)).
+      eapply in_map. eauto.
+    - inv ND; destruct H; eauto. inv H. congruence.
+  Qed.
+
+  Lemma wt_sact_var_exists:
+    forall vvs a t
+           (WTa: wt_sact (Sigma:=Sigma) vvs a t)
+           (VSV: vvs_smaller_variables vvs)
+           (WTV: wt_vvs (Sigma:=Sigma) vvs)
+           v (VIS: var_in_sact a v),
+      In v (map fst vvs).
+  Proof.
+    intros vvs a t WTa VSV WTV. revert a t WTa.
+    induction 1; simpl; intros; eauto; inv VIS; eauto.
+    eapply list_assoc_in_keys; eauto.
+  Qed.
+
+  Lemma inlining_pass_correct:
+    forall sf sf' l
+           (ND: NoDup (map fst (vars sf)))
+           (IP: inlining_pass sf = (sf', l))
+           (VSV: vvs_smaller_variables (vars sf))
+           (WT: wt_vvs (Sigma:=Sigma) (vars sf))
+           v reg (REG: list_assoc (final_values sf) reg = Some v) res
+           (INT: interp_sact (sigma:=sigma) (vars sf) (SVar v) res),
+      (* interp_sact (sigma:=sigma) (vars sf') (SVar v) res \/ *) In (v,res) l.
+  Proof.
+    unfold inlining_pass. intros.
+    repeat destr_in IP. inv IP.
+
+    exploit simplify_vars_correct; eauto.
+    - apply sorted_lt. auto.
+    - eapply Permutation.Permutation_Forall. apply NatSort.Permuted_sort.
+      rewrite Forall_forall.  intros x.  rewrite in_map_iff.
+      intros ((x0 & (?&?)) & EQ & IN). subst. simpl.
+      erewrite in_list_assoc; eauto.
+    - simpl. intros x t y v0 GET VIS. split. auto.
+      eapply Permutation.Permutation_in. apply NatSort.Permuted_sort.
+      exploit WT. apply GET. intro WTy.
+      eapply wt_sact_var_exists; eauto.
+    - intros (IMPL & VVS' & WT' & INTERPl & NIV & _ & IN).
+      edestruct (IN v).
+      eapply Permutation.Permutation_in. apply NatSort.Permuted_sort.
+      inv INT.
+      eapply list_assoc_in_keys; eauto.
+      rewrite Forall_forall in INTERPl.
+      exploit INTERPl. eauto. simpl. intro.
+      inv INT. edestruct IMPL as (y' & GET & INT2). eauto. eauto.
+      inv H0. rewrite GET in H4; inv H4.
+      exploit @interp_sact_determ. apply H5. apply INT2. intro; subst. auto.
+  Qed.
 
   (* Cycles between variables are possible (a variable v can depend on another
      variable which itself depends on v). However, these can only occur in
@@ -171,71 +1323,469 @@ Section SimpleFormInterpretation.
      Note that we don't need our simplifications to be exhaustive: for instance
      we choose to ignore that an and can be short-circuited based on its right
      operand. *)
-  Fixpoint simplify_uact (ua: uact) : uact :=
+  Fixpoint simplify_sact (ua: sact) : sact :=
     match ua with
-    | UIf cond tb fb =>
-      let cond' := simplify_uact cond in
-      let tb' := simplify_uact tb in
-      let fb' := simplify_uact fb in
-      if (negb (contains_vars cond')) then
-        match interp_action r sigma [] log_empty log_empty cond' with
-        | Some (_, Bits 1 [true], _) => tb'
-        | Some (_, Bits 1 [false], _) => fb'
-        | _ => UVar "ERROR cond" (* Should never happen *)
-        end
-      else UIf cond' tb' fb'
-    | UBinop ufn a1 a2 =>
-      let a1' := simplify_uact a1 in
-      let a2' := simplify_uact a2 in
-      if negb (contains_vars a1') then
-        match ufn with
-        | PrimUntyped.UBits2 PrimUntyped.UAnd =>
-          match interp_action r sigma [] log_empty log_empty a1' with
-          | Some (_, Bits 1 [false], _) => const_false
-          | Some (_, Bits 1 [true], _) => a2'
-          | _ => UVar "ERROR binop and" (* Should never happen *)
+    | SIf cond tb fb =>
+      let cond' := simplify_sact cond in
+      let tb' := simplify_sact tb in
+      let fb' := simplify_sact fb in
+      match eval_sact_no_vars cond' with
+      | Some (Bits 1 [true]) => tb'
+      | Some (Bits 1 [false]) => fb'
+      | _ => SIf cond' tb' fb'
+      end
+    | SBinop ufn a1 a2 =>
+      let a1' := simplify_sact a1 in
+      let a2' := simplify_sact a2 in
+      match ufn with
+      | PrimUntyped.UBits2 PrimUntyped.UAnd =>
+          match eval_sact_no_vars a1', eval_sact_no_vars a2' with
+          | Some (Bits 1 [false]), _ => const_false
+          | Some (Bits 1 [true]), _ => a2'
+          | _, Some (Bits 1 [false]) => const_false
+          | _, Some (Bits 1 [true]) => a1'
+          | _, _ => SBinop ufn a1' a2'
           end
         | PrimUntyped.UBits2 PrimUntyped.UOr =>
-          match interp_action r sigma [] log_empty log_empty a1' with
-          | Some (_, Bits 1 [true], _) => const_true
-          | Some (_, Bits 1 [false], _) => a2'
-          | _ => UVar "ERROR binop or" (* Should never happen *)
+          match eval_sact_no_vars a1', eval_sact_no_vars a2' with
+          | Some (Bits 1 [true]), _
+          | _, Some (Bits 1 [true]) => const_true
+          | Some (Bits 1 [false]), _  => a2'
+          | _, _ => SBinop ufn a1' a2'
           end
-        | _ => UBinop ufn a1' a2'
+        | _ => SBinop ufn a1' a2'
         end
-      else UBinop ufn a1' a2'
-    | UUnop ufn a => (* Perhaps not strictly required *)
-        UUnop ufn (simplify_uact a)
-    | _ => ua
+    | SUnop ufn a => (* Perhaps not strictly required *)
+        let a := simplify_sact a in
+        match ufn with
+        | PrimUntyped.UBits1 PrimUntyped.UNot =>
+            match eval_sact_no_vars a with
+            | Some (Bits 1 [b]) => SConst (Bits 1 [negb b])
+            | _ => SUnop ufn a
+            end
+        | _ => SUnop ufn a
+        end
+    | SExternalCall ufn a => SExternalCall ufn (simplify_sact a)
+    | SVar _
+    | SConst _ => ua
     end.
 
-  Definition expr_simplification_pass (sf: @simple_form pos_t reg_t ext_fn_t)
-  : simple_form := {|
-    final_values := final_values sf;
-    vars := map (fun '(vn, vu) => (vn, simplify_uact vu)) (vars sf);
-    external_calls :=
-      map
-        (fun '(efn, ei) => (efn, {|
-          econd := simplify_uact (econd ei); earg := simplify_uact (earg ei);
-          ebind := ebind ei; |}))
-        (external_calls sf) |}.
+  Lemma eval_sact_eval_sact_no_vars:
+    forall vvs n a res res2,
+      eval_sact vvs a n = Some res ->
+      eval_sact_no_vars a = Some res2 ->
+      res = res2.
+  Proof.
+    induction n; simpl; intros; eauto. inv H.
+    unfold opt_bind in H.
+    repeat destr_in H; inv H; simpl in H0; inv H0; eauto.
+    - unfold opt_bind in H1. destr_in H1.
+      exploit IHn. apply Heqo. eauto. intros <-.
+      exploit IHn. apply H2. eauto. auto. inv H1.
+    - unfold opt_bind in H1. destr_in H1.
+      exploit IHn. apply Heqo. eauto. intros <-.
+      exploit IHn. apply H2. eauto. auto. inv H1.
+    - unfold opt_bind in H1. destr_in H1.
+      exploit IHn. apply Heqo. eauto. intros <-.
+      congruence. congruence.
+    - unfold opt_bind in H1. destr_in H1.
+      exploit IHn. apply Heqo. eauto.
+      destr_in H1.
+      exploit IHn. apply Heqo0. eauto. intros. congruence. congruence. congruence.
+    - unfold opt_bind in H1. destr_in H1.
+      exploit IHn. apply Heqo. eauto. intro; subst. congruence. congruence.
+  Qed.
 
-  Definition simplification_pass (sf: @simple_form pos_t reg_t ext_fn_t)
-  : simple_form * list (string * val)  :=
+  Lemma simplify_unop_cases:
+    forall ufn a a' ,
+      simplify_sact (SUnop ufn a) = a' ->
+      (exists b, ufn = PrimUntyped.UBits1 PrimUntyped.UNot /\ eval_sact_no_vars (simplify_sact a) = Some (Bits 1 [b]) /\ a' = SConst (Bits 1 [negb b]))
+      \/ a' = SUnop ufn (simplify_sact a).
+  Proof.
+    intros. simpl in H. subst. repeat destr; eauto.
+  Qed.
+
+  Lemma simplify_bnop_cases:
+    forall ufn a1 a2 a' ,
+      simplify_sact (SBinop ufn a1 a2) = a' ->
+      a' = SBinop ufn (simplify_sact a1) (simplify_sact a2)
+      \/ (ufn = PrimUntyped.UBits2 PrimUntyped.UAnd
+          /\ ((eval_sact_no_vars (simplify_sact a1) = Some (Bits 1 [true])
+               /\ a' = simplify_sact a2)
+              \/ (eval_sact_no_vars (simplify_sact a1) = Some (Bits 1 [false])
+                  /\ a' = const_false)
+              \/ (eval_sact_no_vars (simplify_sact a2) = Some (Bits 1 [true])
+                  /\ a' = simplify_sact a1)
+              \/ (eval_sact_no_vars (simplify_sact a2) = Some (Bits 1 [false])
+                  /\ a' = const_false)))
+      \/ (ufn = PrimUntyped.UBits2 PrimUntyped.UOr
+          /\ ((eval_sact_no_vars (simplify_sact a1) = Some (Bits 1 [true])
+               /\ a' = const_true)
+              \/ (eval_sact_no_vars (simplify_sact a1) = Some (Bits 1 [false])
+                  /\ a' = simplify_sact a2)
+              \/ (eval_sact_no_vars (simplify_sact a2) = Some (Bits 1 [true])
+                  /\ a' = const_true)
+              \/ (eval_sact_no_vars (simplify_sact a2) = Some (Bits 1 [false])
+                  /\ a' = simplify_sact a1))).
+  Proof.
+    intros. simpl in H. subst.
+    repeat destr; intuition eauto.
+  Qed.
+
+  Lemma eval_sact_wt:
+    forall vvs (WT: wt_vvs (Sigma:=Sigma) vvs) n a r t (WTa: wt_sact (Sigma:=Sigma) vvs a t)
+           (EVAL: eval_sact vvs a n = Some r),
+      wt_val t r.
+  Proof.
+    induction n; simpl; intros; eauto. inv EVAL.
+    unfold opt_bind in EVAL; repeat destr_in EVAL; inv EVAL; inv WTa; eauto.
+    - rewrite Heqo in H1; inv H1.
+      eapply IHn; eauto.
+    - eapply Wt.wt_unop_sigma1; eauto.
+    - eapply Wt.wt_binop_sigma1; eauto.
+  Qed.
+
+  Lemma simplify_sact_correct:
+    forall vvs (WTV: wt_vvs (Sigma:=Sigma) vvs) n a res t,
+      wt_sact (Sigma:=Sigma) vvs a t ->
+      eval_sact vvs a n = Some res ->
+      eval_sact vvs (simplify_sact a) n = Some res.
+  Proof.
+    induction n; intros a res t WT EVAL; eauto.
+    simpl in EVAL.
+    unfold opt_bind in EVAL.
+    repeat destr_in EVAL; inv EVAL; auto.
+    - simpl. rewrite Heqo; eauto.
+    - inv WT.
+      simpl.
+      destruct (eval_sact_no_vars (simplify_sact s1)) eqn:?.
+      eapply eval_sact_eval_sact_no_vars in Heqo0; eauto. subst.
+      transitivity (eval_sact vvs (simplify_sact s2) (S n)). reflexivity.
+      exploit IHn. 2: apply H0. eauto. intro ES. exploit eval_sact_more_fuel. apply ES.
+      2: intro ES'; rewrite ES'. lia. eauto.
+      erewrite IHn. 2-3: eauto. simpl.
+      erewrite IHn; eauto.
+    - inv WT.
+      simpl.
+      destruct (eval_sact_no_vars (simplify_sact s1)) eqn:?.
+      eapply eval_sact_eval_sact_no_vars in Heqo0; eauto. subst.
+      transitivity (eval_sact vvs (simplify_sact s3) (S n)). reflexivity.
+      exploit IHn. 2: apply H0. eauto. intro ES. exploit eval_sact_more_fuel. apply ES.
+      2: intro ES'; rewrite ES'. lia. eauto.
+      erewrite IHn. 2-3: eauto. simpl.
+      erewrite IHn; eauto.
+    - destruct (simplify_unop_cases ufn1 s _ eq_refl) as [(b & EQ & ESNV & EQ')|EQ].
+      + inv WT.
+        rewrite EQ'. simpl.
+        exploit eval_sact_eval_sact_no_vars. 2: eauto. eapply IHn. eauto. eauto. intros ->.
+        simpl. auto.
+      + inv WT; rewrite EQ. simpl. erewrite IHn; simpl; eauto.
+    - inv WT.
+      exploit eval_sact_wt. 3: apply Heqo. all: eauto.
+      exploit eval_sact_wt. 3: apply Heqo0. all: eauto.
+      intros WTv2 WTv1.
+      exploit Wt.wt_binop_sigma1. eauto. eauto. eauto. eauto. intro WTres.
+      eapply IHn in Heqo; eauto.
+      eapply IHn in Heqo0; eauto.
+
+      destruct (simplify_bnop_cases ufn2 s1 s2 _ eq_refl) as
+        [EQ|[(ufneq & [(ESNV & EQ)|[(ESNV & EQ)|[(ESNV & EQ)|(ESNV & EQ)]]])
+            |(ufneq & [(ESNV & EQ)|[(ESNV & EQ)|[(ESNV & EQ)|(ESNV & EQ)]]])]]; rewrite EQ; clear EQ.
+      + simpl. rewrite Heqo, Heqo0.  reflexivity.
+      + exploit eval_sact_eval_sact_no_vars. apply Heqo. apply ESNV. intros ->.
+        inv WTv1. inv H6.
+        apply wt_val_bool in WTv2.
+        apply wt_val_bool in WTres.
+        destruct WTv2, WTres. subst.
+        erewrite eval_sact_more_fuel. 2: eauto. simpl. auto. lia.
+      + exploit eval_sact_eval_sact_no_vars. apply Heqo. apply ESNV. intros ->.
+        inv WTv1. inv H6.
+        apply wt_val_bool in WTv2.
+        apply wt_val_bool in WTres.
+        destruct WTv2, WTres. subst.
+        simpl. auto.
+      + exploit eval_sact_eval_sact_no_vars. 2: apply ESNV. eauto. intros ->.
+        inv WTv2. inv H6.
+        apply wt_val_bool in WTv1.
+        apply wt_val_bool in WTres.
+        destruct WTv1, WTres. subst.
+        erewrite eval_sact_more_fuel. 2: eauto. simpl. rewrite andb_true_r; auto. lia.
+      + exploit eval_sact_eval_sact_no_vars. 2: apply ESNV. eauto. intros ->.
+        inv WTv2. inv H6.
+        apply wt_val_bool in WTv1.
+        apply wt_val_bool in WTres.
+        destruct WTv1, WTres. subst.
+        simpl. rewrite andb_false_r; auto.
+      + exploit eval_sact_eval_sact_no_vars. 2: apply ESNV. eauto. intros ->.
+        inv WTv1. inv H6.
+        apply wt_val_bool in WTv2.
+        apply wt_val_bool in WTres.
+        destruct WTv2, WTres. subst. simpl; auto.
+      + exploit eval_sact_eval_sact_no_vars. 2: apply ESNV. eauto. intros ->.
+        inv WTv1. inv H6.
+        apply wt_val_bool in WTv2.
+        apply wt_val_bool in WTres.
+        destruct WTv2, WTres. subst.
+        erewrite eval_sact_more_fuel. 2: eauto. simpl. auto. lia.
+      + exploit eval_sact_eval_sact_no_vars. 2: apply ESNV. eauto. intros ->.
+        inv WTv2. inv H6.
+        apply wt_val_bool in WTv1.
+        apply wt_val_bool in WTres.
+        destruct WTv1, WTres. subst. simpl. rewrite orb_true_r; auto.
+      + exploit eval_sact_eval_sact_no_vars. 2: apply ESNV. eauto. intros ->.
+        inv WTv2. inv H6.
+        apply wt_val_bool in WTv1.
+        apply wt_val_bool in WTres.
+        destruct WTv1, WTres. subst.
+        erewrite eval_sact_more_fuel. 2: eauto. simpl. rewrite orb_false_r; auto. lia.
+    - simpl. inv WT;  erewrite IHn; simpl; eauto.
+  Qed.
+
+  Definition expr_simplification_pass (sf: simple_form)
+    : simple_form :=
+    {|
+      final_values := final_values sf;
+      vars := map (fun '(vn, (t,vu)) => (vn, (t, simplify_sact vu))) (vars sf);
+    |}.
+
+  Lemma wt_sact_replace_vars_gen:
+    forall vvs f a t,
+      wt_sact (Sigma:=Sigma) vvs a t ->
+      wt_sact (Sigma:=Sigma) (map (fun '(n,(t,u)) => (n,(t,f u))) vvs) a t.
+  Proof.
+    induction 1; simpl; intros; eauto.
+    - econstructor.
+      erewrite list_assoc_map with (g := fun '(t,a) => (t, f a)). 2: intros; repeat destr.
+      rewrite H. reflexivity.
+    - econstructor; eauto.
+    - econstructor; eauto.
+    - econstructor; eauto.
+    - econstructor; eauto.
+    - econstructor; eauto.
+  Qed.
+
+  Lemma wt_vvs_replace_gen:
+    forall vvs f,
+      wt_vvs (Sigma:=Sigma) vvs ->
+      (forall t u, wt_sact (Sigma:=Sigma) vvs u t -> wt_sact (Sigma:=Sigma) vvs (f u) t) ->
+      wt_vvs (Sigma:=Sigma) (map (fun '(n,(t,u)) => (n,(t,f u)))vvs).
+  Proof.
+    unfold wt_vvs; intros.
+    setoid_rewrite list_assoc_map with (g:= fun '(t,a) => (t, f a)) in H1.
+    2: intros; repeat destr.
+    unfold option_map in H1; repeat destr_in H1; inv H1.
+    eapply wt_sact_replace_vars_gen. eapply H0; eauto.
+  Qed.
+
+  Lemma simplify_sact_wt:
+    forall vvs a t,
+      wt_sact (Sigma:=Sigma) vvs a t ->
+      wt_sact (Sigma:=Sigma) vvs (simplify_sact a) t.
+  Proof.
+    induction 1; simpl; intros; eauto.
+    - econstructor; eauto.
+    - econstructor; eauto.
+    - destr. exploit eval_sact_no_vars_wt.  2: apply Heqo. eauto.
+      intro WT. apply wt_val_bool in WT. destruct WT.  subst. destr.
+      econstructor; eauto.
+    - repeat destr; try now (econstructor; eauto).
+      subst.
+      exploit eval_sact_no_vars_wt.  2: apply Heqo. eauto.
+      intro WT. inv WT. inv H0. repeat econstructor.
+    - destr; try now (econstructor; eauto).
+      destr; try now (econstructor; eauto).
+      + destr; try now (econstructor; eauto).
+        exploit eval_sact_no_vars_wt.  2: apply Heqo. eauto.
+        intro WT1. inv H1. inv WT1.
+        destruct (eval_sact_no_vars (simplify_sact a2)) eqn:?.
+        exploit eval_sact_no_vars_wt.  2: apply Heqo0. eauto.
+        intro WT2. inv WT2.
+        destr; try now (econstructor; eauto). repeat econstructor; eauto.
+        destruct bs, bs0; simpl in *; try lia.
+        destr; try now (econstructor; eauto).
+        destruct bs, bs0; simpl in *; try lia.
+        destr; eauto. repeat econstructor. repeat econstructor; eauto.
+        repeat destr; try now (repeat econstructor; eauto).
+        destr; try now (repeat econstructor; eauto).
+        exploit eval_sact_no_vars_wt.  2: apply Heqo0. eauto.
+        intro WT2. inv H1. inv WT2.
+        repeat destr; try now (repeat econstructor; eauto).
+      + destr; try now (econstructor; eauto).
+        exploit eval_sact_no_vars_wt.  2: apply Heqo. eauto.
+        intro WT1. inv H1. inv WT1.
+        destruct (eval_sact_no_vars (simplify_sact a2)) eqn:?.
+        exploit eval_sact_no_vars_wt.  2: apply Heqo0. eauto.
+        intro WT2. inv WT2.
+        repeat destr; try now (repeat econstructor; eauto).
+        repeat destr; try now (repeat econstructor; eauto).
+        destr; try now (repeat econstructor; eauto).
+        exploit eval_sact_no_vars_wt.  2: apply Heqo0. eauto.
+        intro WT2. inv H1. inv WT2.
+        repeat destr; try now (repeat econstructor; eauto).
+    - econstructor. eauto.
+  Qed.
+
+  Lemma simplify_sact_vars_correct_preserves_wt:
+    forall sf (WTV: wt_vvs (Sigma:=Sigma) (vars sf)) sf' (ESP: expr_simplification_pass sf = sf'),
+      wt_vvs (Sigma:=Sigma) (vars sf').
+  Proof.
+    intros; subst.
+    simpl. eapply wt_vvs_replace_gen. auto.
+    intros. eapply simplify_sact_wt. auto.
+  Qed.
+
+  Lemma interp_map_vvs:
+    forall vvs (VSV: vvs_smaller_variables vvs) (WTvvs: wt_vvs (Sigma:=Sigma) vvs)
+           a
+           t (WTa: wt_sact (Sigma:=Sigma) vvs a t)
+           (* (NVa: ~ var_in_sact a v) *) res f
+           (VARS: forall v s, var_in_sact (f s) v -> var_in_sact s v)
+           (* (WTf: forall s t, wt_sact (Sigma:=Sigma) vvs s t ->  wt_sact (Sigma:=Sigma) vvs (f s) t) *)
+           (* (WTf: forall s t, wt_sact (Sigma:=Sigma) vvs s t ->  wt_sact (Sigma:=Sigma) (map (fun '(n,(t,a)) => (n, (t, f a))) vvs) s t) *)
+           (WTf2: forall s t, wt_sact (Sigma:=Sigma) vvs s t ->  wt_sact (Sigma:=Sigma) vvs (f s) t)
+           (CORRECT: forall vvs s t n res,
+               wt_vvs (Sigma:=Sigma) vvs ->
+               wt_sact (Sigma:=Sigma) vvs s t ->
+               eval_sact vvs s n = Some res ->
+               eval_sact vvs (f s) n = Some res
+           )
+    ,
+      interp_sact (sigma:=sigma) vvs a res ->
+      interp_sact (sigma:=sigma) (map (fun '(n,(t,a)) => (n, (t, f a))) vvs) a res.
+  Proof.
+    intros.
+    eapply interp_sact_eval_sact in H; eauto.
+    revert H. generalize (S (max_var vvs) + vvs_size vvs (S (max_var vvs)) + size_sact a). intros.
+    eapply eval_sact_interp_sact with (fuel:=n).
+    revert a res H t WTa.
+    
+    induction n. simpl; intros; eauto.
+    simpl. unfold opt_bind.
+    intros a res EVAL.
+    destr_in EVAL.
+    - repeat destr_in EVAL. 2: inv EVAL.
+      rewrite list_assoc_map with (g:=fun '(t,a) => (t, f a)). rewrite Heqo. simpl.
+      intros; eapply IHn. eauto. eapply WTvvs in Heqo. eapply WTf2. eauto.
+      intros; repeat destr.
+    - auto.
+    - intros t WTa; inv WTa.
+      destr_in EVAL. 2: inv EVAL.
+      erewrite IHn; eauto.
+      repeat destr_in EVAL; try now inv EVAL. subst.
+      eapply IHn; eauto.
+      eapply IHn; eauto.
+    - intros t WTa; inv WTa.
+      destr_in EVAL. 2: inv EVAL.
+      erewrite IHn; eauto.
+    - intros t WTa; inv WTa.
+      destr_in EVAL. 2: inv EVAL.
+      destr_in EVAL. 2: inv EVAL.
+      erewrite IHn; eauto.
+      erewrite IHn; eauto.
+    - intros t WTa; inv WTa.
+      destr_in EVAL. 2: inv EVAL.
+      erewrite IHn; eauto.
+  Qed.
+
+  Lemma simplify_sact_vars:
+    forall (v : nat) (s : SimpleForm.sact),
+      var_in_sact (simplify_sact s) v -> var_in_sact s v.
+  Proof.
+    induction s; intros; eauto.
+    -
+      Lemma simplify_if_cases s1 s2 s3 s:
+        simplify_sact (SIf s1 s2 s3) = s ->
+        s = SIf (simplify_sact s1) (simplify_sact s2) (simplify_sact s3)
+        \/ (eval_sact_no_vars (simplify_sact s1) = Some (Bits 1 [true]) /\ s = simplify_sact s2)
+        \/ (eval_sact_no_vars (simplify_sact s1) = Some (Bits 1 [false]) /\ s = simplify_sact s3).
+      Proof.
+        intros <-. simpl. repeat destr; auto.
+      Qed.
+      destruct (simplify_if_cases s1 s2 s3 _ eq_refl) as [EQ|[(ESNV & EQ)|(ESNV & EQ)]];
+        rewrite EQ in H; clear EQ.
+      + inv H.
+        eapply var_in_if_cond; eauto.
+        eapply var_in_if_true; eauto.
+        eapply var_in_if_false; eauto.
+      + eapply var_in_if_true; eauto.
+      + eapply var_in_if_false; eauto.
+    - destruct (simplify_unop_cases ufn1 s _ eq_refl) as [(b & EQ & ESNV & EQ')|EQ']; rewrite EQ' in H; clear EQ'. inv H. inv H.
+      eapply var_in_sact_unop; eauto.
+    - destruct (simplify_bnop_cases ufn2 s1 s2 _ eq_refl) as
+        [EQ|[(ufneq & [(ESNV & EQ)|[(ESNV & EQ)|[(ESNV & EQ)|(ESNV & EQ)]]])
+            |(ufneq & [(ESNV & EQ)|[(ESNV & EQ)|[(ESNV & EQ)|(ESNV & EQ)]]])]]; rewrite EQ in H; clear EQ.
+      + inv H. eapply var_in_sact_binop_1; eauto.
+        eapply var_in_sact_binop_2; eauto.
+      + eapply var_in_sact_binop_2; eauto.
+      + inv H.
+      + eapply var_in_sact_binop_1; eauto.
+      + inv H.
+      + inv H.
+      + eapply var_in_sact_binop_2; eauto.
+      + inv H.
+      + eapply var_in_sact_binop_1; eauto.
+    - inv H. eapply var_in_sact_external; eauto.
+  Qed.
+
+  Lemma simplify_sact_vars_correct:
+    forall sf (VSV: vvs_smaller_variables (vars sf))
+           (WTV: wt_vvs (Sigma:=Sigma) (vars sf)) sf' (ESP: expr_simplification_pass sf = sf')
+           x t y res
+           (GET: list_assoc (vars sf) x = Some (t, y))
+           (INT: interp_sact (sigma:=sigma) (vars sf) y res),
+    exists y' ,
+      list_assoc (vars sf') x = Some (t, y') /\
+        interp_sact (sigma:=sigma) (vars sf') y' res.
+  Proof.
+    intros. subst. simpl.
+    setoid_rewrite list_assoc_map with (g:= fun '(t,a) => (t, simplify_sact a)). 2: intros; repeat destr.
+    setoid_rewrite GET. simpl. eexists; split; eauto.
+    eapply interp_map_vvs; eauto.
+    eapply simplify_sact_wt; eauto.
+    eapply simplify_sact_vars; eauto.
+    eapply simplify_sact_wt; eauto.
+    intros vvs s t0 n res0 WTVVS. eapply simplify_sact_correct. auto.
+
+    eapply interp_sact_eval_sact in INT; eauto.
+    revert INT.
+    generalize (S (max_var (vars sf)) + vvs_size (vars sf) (S (max_var (vars sf))) +
+                  size_sact y). intros.
+    eapply simplify_sact_correct in INT; eauto.
+    eapply eval_sact_interp_sact; eauto.
+  Qed.
+
+  Definition simplification_pass (sf: simple_form)
+  : simple_form * list (nat * val)  :=
     inlining_pass (expr_simplification_pass sf).
 
-  Fixpoint simplify (sf: @simple_form pos_t reg_t ext_fn_t) (fuel: nat)
-  : list (string * val) :=
-    match fuel with
-    | O => [] (* Should never happen *)
-    | S f' =>
-      let (sf', vals) := simplification_pass sf in
-      vals++(simplify sf' f')
-    end.
+  (* Lemma simplification_pass_correct: *)
+  (*   forall sf (VSV: vvs_smaller_variables (vars sf)) *)
+  (*          (WTV: wt_vvs (Sigma:=Sigma) (vars sf)) *)
+  (*          sf' l *)
+  (*          (SP: simplification_pass sf = (sf', l)) *)
+  (*          x t y res *)
+  (*          (GET: list_assoc (vars sf) x = Some (t, y)) *)
+  (*          (INT: interp_sact (sigma:=sigma) (vars sf) y res), *)
+  (*   exists y' , *)
+  (*     list_assoc (vars sf') x = Some (t, y') /\ *)
+  (*       interp_sact (sigma:=sigma) (vars sf') y' res. *)
+  (* Proof. *)
+
+
+  (* Fixpoint simplify (sf: simple_form) (fuel: nat) *)
+  (* : list (nat * val) := *)
+  (*   match fuel with *)
+  (*   | O => [] *)
+  (*   | S f' => *)
+  (*     let (sf', vals) := simplification_pass sf in *)
+  (*     vals++(simplify sf' f') *)
+  (*   end. *)
+
+
 
   Definition interp_cycle (sf: @simple_form pos_t reg_t ext_fn_t) : UREnv :=
     let fenv :=
-      simplify sf (List.length (vars sf) + List.length (external_calls sf))
+      simplify sf (List.length (vars sf))
     in
     (* No need to explicitly inline read0s: delegated to interp_action *)
     fold_left
@@ -250,7 +1800,7 @@ Section SimpleFormInterpretation.
 
   Lemma normal_form_ok:
     forall
-      (r: UREnv) (sigma: ext_funs_defs) (rules: rule_name_t -> uact)
+      (r: UREnv) (sigma: ext_funs_defs) (rules: rule_name_t -> sact)
       (s: schedule) (p: pos_t)
       (TA:
         forall rule, exists tcr,
@@ -262,7 +1812,7 @@ Section SimpleFormInterpretation.
   Admitted.
   (* Lemma simple_form_ok: *)
   (*   forall *)
-  (*     (r: UREnv) (sigma: ext_funs_defs) (rules: rule_name_t -> uact) *)
+  (*     (r: UREnv) (sigma: ext_funs_defs) (rules: rule_name_t -> sact) *)
   (*     (s: schedule) (p: pos_t) *)
   (*     (TA: *)
   (*       forall rule, exists tcr, *)
